Begin pushing typing invariant through linking proof

core/effect_simulations.v
@@ -19,57 +19,49 @@ Require Import reach.
 
 Module SM_simulation. Section SharedMemory_simulation_inject. 
 
-  Context {F1 V1 C1 F2 V2 C2 : Type}
-          (Sem1 : @EffectSem (Genv.t F1 V1) C1)
-          (Sem2 : @EffectSem (Genv.t F2 V2) C2)
-          (ge1 : Genv.t F1 V1)
-          (ge2 : Genv.t F2 V2).
+Context 
+  {F1 V1 C1 F2 V2 C2 : Type}
+  (Sem1 : @EffectSem (Genv.t F1 V1) C1)
+  (Sem2 : @EffectSem (Genv.t F2 V2) C2)
+  (ge1 : Genv.t F1 V1)
+  (ge2 : Genv.t F2 V2).
 
-  Record SM_simulation_inject := 
-  { core_data : Type;
-    match_state : core_data -> SM_Injection -> C1 -> mem -> C2 -> mem -> Prop;
-    core_ord : core_data -> core_data -> Prop;
-    core_ord_wf : well_founded core_ord;
+Record SM_simulation_inject := 
+{ core_data : Type
+; match_state : core_data -> SM_Injection -> C1 -> mem -> C2 -> mem -> Prop
+; core_ord : core_data -> core_data -> Prop
+; core_ord_wf : well_founded core_ord
 
-    match_sm_wd : forall d mu c1 m1 c2 m2, 
-          match_state d mu c1 m1 c2 m2 ->
-          SM_wd mu;
+; match_sm_wd : 
+    forall d mu c1 m1 c2 m2, 
+    match_state d mu c1 m1 c2 m2 -> SM_wd mu
 
-    genvs_dom_eq: genvs_domain_eq ge1 ge2;
+; genvs_dom_eq : genvs_domain_eq ge1 ge2
 
-(*  The match_genv condition below used to be formulated as:
+; match_genv : 
+    forall d mu c1 m1 c2 m2 (MC : match_state d mu c1 m1 c2 m2),
+    meminj_preserves_globals ge1 (extern_of mu) /\
+    (forall b, isGlobalBlock ge1 b = true -> frgnBlocksSrc mu b = true)
 
-      match_genv: forall d mu c1 m1 c2 m2,  match_state d mu c1 m1 c2 m2 -> 
-          meminj_preserves_globals ge1 (foreign_of mu); 
+; match_visible : 
+    forall d mu c1 m1 c2 m2, 
+    match_state d mu c1 m1 c2 m2 -> 
+    REACH_closed m1 (vis mu)
 
-    The following formulation using extern_of is slightly stronger,
-    since it requires that the third condition of
-    mem-inj_preserves_globals be satisfied for all of extern_of, bit
-    just foreign_of, so is preserved by extern_incr and the adaptation
-    of frgSrc by replaces_externs in rule afterExternal. It is also
-    equivalent to a formulation that uses as_inj instead of extern_of;
-    see Lemma match_genv_meminj_preserves_extern_iff_all in
-    effect_properties.v *)
+; match_restrict : 
+    forall d mu c1 m1 c2 m2 X, 
+    match_state d mu c1 m1 c2 m2 -> 
+    (forall b, vis mu b = true -> X b = true) ->
+    REACH_closed m1 X ->
+    match_state d (restrict_sm mu X) c1 m1 c2 m2
 
-    match_genv : forall d mu c1 m1 c2 m2 (MC:match_state d mu c1 m1 c2 m2),
-          meminj_preserves_globals ge1 (extern_of mu) /\
-          (forall b, isGlobalBlock ge1 b = true -> frgnBlocksSrc mu b = true); 
+; match_validblocks : 
+    forall d mu c1 m1 c2 m2, 
+    match_state d mu c1 m1 c2 m2 ->
+    sm_valid mu m1 m2
 
-    match_visible : forall d mu c1 m1 c2 m2, 
-          match_state d mu c1 m1 c2 m2 -> 
-          REACH_closed m1 (vis mu);
 
-    match_restrict : forall d mu c1 m1 c2 m2 X, 
-          match_state d mu c1 m1 c2 m2 -> 
-          (forall b, vis mu b = true -> X b = true) ->
-          REACH_closed m1 X ->
-          match_state d (restrict_sm mu X) c1 m1 c2 m2;
-
-    match_validblocks : forall d mu c1 m1 c2 m2, 
-          match_state d mu c1 m1 c2 m2 ->
-          sm_valid mu m1 m2;  
-
-  core_initial : 
+; core_initial : 
     forall v vals1 c1 m1 j vals2 m2 DomS DomT,
     initial_core Sem1 ge1 v vals1 = Some c1 ->
     Mem.inject j m1 m2 -> 
@@ -99,90 +91,68 @@ Module SM_simulation. Section SharedMemory_simulation_inject.
          (initial_SM DomS DomT 
            (REACH m1 (fun b => isGlobalBlock ge1 b || getBlocks vals1 b)) 
            (REACH m2 (fun b => isGlobalBlock ge2 b || getBlocks vals2 b)) j)
-         c1 m1 c2 m2;
+         c1 m1 c2 m2
 
-    core_diagram : 
-      forall st1 m1 st1' m1', 
-        corestep Sem1 ge1 st1 m1 st1' m1' ->
-      forall cd st2 mu m2,
-        match_state cd mu st1 m1 st2 m2 ->
-        exists st2', exists m2', exists cd', exists mu',
-          intern_incr mu mu' /\
-          sm_inject_separated mu mu' m1 m2 /\
-          sm_locally_allocated mu mu' m1 m2 m1' m2' /\ 
-          match_state cd' mu' st1' m1' st2' m2' /\
-          ((corestep_plus Sem2 ge2 st2 m2 st2' m2') \/
-            corestep_star Sem2 ge2 st2 m2 st2' m2' /\
-            core_ord cd' cd);
 
-        (* One would suspect that we could add the following
-           confinement guarantees to this rule:
- 
-          /\ Mem.unchanged_on (fun b2 ofs => 
-                   extBlocksTgt mu b2 = true /\
-                   ~ exists b1 d, foreign_of mu b1=Some (b2,d)) m2 m2' 
-          /\ forall b ofs, 
-               Mem.unchanged_on (fun b' ofs' => b'=b /\ ofs'=ofs) m1 m1' ->
-               forall b2 d, 
-                  foreign_of mu b = Some(b2,d) -> 
-                  Mem.unchanged_on (fun b' ofs' => b'=b2 /\ ofs'=ofs+d) m2 m2'
- 
-         Indeed, as RGTgt_multicoreNOEFFECTS at the end of this file
-         shows, these guarantees suffice for establishing the
-         afterEtxernal-rely (under the mild axiom
-         DECIBILITYAXIOM). However, these guarantees cannot be pushed
-         through the transitivity proof (inductive step of "case1"),
-         since Mem_unchanged_on does not decompose, ie for step m m'
-         /\ step m' m'' /\ UnchOn P m m'' does not imply UnchOn P m m'
-         /\ UnchOn P m' m''. But such decomposition would be needed to
-         apply the induction hypotheses of core_diagram in file
-         effect_corediagram_trans.v The advantage of/reason for using
-         effects is to have such decomposition, as step m m' /\ step
-         m' m'' /\ Estep E m m'' does imply Estep E m m' /\ Estep E m' m''. *)
+; core_diagram : 
+    forall st1 m1 st1' m1', 
+    corestep Sem1 ge1 st1 m1 st1' m1' ->
+    forall cd st2 mu m2,
+    match_state cd mu st1 m1 st2 m2 ->
+    exists st2', exists m2', exists cd', exists mu',
+      intern_incr mu mu' 
+      /\ sm_inject_separated mu mu' m1 m2 
+      /\ sm_locally_allocated mu mu' m1 m2 m1' m2' 
+      /\ match_state cd' mu' st1' m1' st2' m2'
+      /\ ((corestep_plus Sem2 ge2 st2 m2 st2' m2') \/
+           corestep_star Sem2 ge2 st2 m2 st2' m2' /\
+           core_ord cd' cd) 
 
-      effcore_diagram : 
-      forall st1 m1 st1' m1' U1, 
-        effstep Sem1 ge1 U1 st1 m1 st1' m1' ->
 
-      forall cd st2 mu m2
-        (UHyp: forall b1 z, U1 b1 z = true -> vis mu b1 = true),
-        match_state cd mu st1 m1 st2 m2 ->
-        exists st2', exists m2', exists cd', exists mu',
-          intern_incr mu mu' /\
-          sm_inject_separated mu mu' m1 m2 /\
-          sm_locally_allocated mu mu' m1 m2 m1' m2' /\ 
-          match_state cd' mu' st1' m1' st2' m2' /\
-          exists U2,              
-            ((effstep_plus Sem2 ge2 U2 st2 m2 st2' m2' \/
-              (effstep_star Sem2 ge2 U2 st2 m2 st2' m2' /\
-               core_ord cd' cd)) /\
-            forall b ofs, 
-              U2 b ofs = true -> 
-              (visTgt mu b = true /\
-               (locBlocksTgt mu b = false ->
-                exists b1 delta1, 
-                  foreign_of mu b1 = Some(b,delta1) /\
-                  U1 b1 (ofs-delta1) = true /\ 
-                  Mem.perm m1 b1 (ofs-delta1) Max Nonempty)));
+; effcore_diagram : 
+    forall st1 m1 st1' m1' U1, 
+    effstep Sem1 ge1 U1 st1 m1 st1' m1' ->
+
+    forall cd st2 mu m2
+           (UHyp: forall b1 z, U1 b1 z = true -> vis mu b1 = true),
+    match_state cd mu st1 m1 st2 m2 ->
+    exists st2', exists m2', exists cd', exists mu',
+    intern_incr mu mu' 
+    /\ sm_inject_separated mu mu' m1 m2 
+    /\ sm_locally_allocated mu mu' m1 m2 m1' m2' 
+    /\ match_state cd' mu' st1' m1' st2' m2' 
+    /\ exists U2,              
+       ((effstep_plus Sem2 ge2 U2 st2 m2 st2' m2' 
+        \/ (effstep_star Sem2 ge2 U2 st2 m2 st2' m2' /\ core_ord cd' cd))
+       /\ forall b ofs, 
+          U2 b ofs = true -> 
+          visTgt mu b = true
+          /\ (locBlocksTgt mu b = false ->
+              exists b1 delta1, 
+              foreign_of mu b1 = Some(b,delta1)
+              /\ U1 b1 (ofs-delta1) = true 
+              /\ Mem.perm m1 b1 (ofs-delta1) Max Nonempty))
+
       
-    core_halted : forall cd mu c1 m1 c2 m2 v1,
-      match_state cd mu c1 m1 c2 m2 ->
-      halted Sem1 c1 = Some v1 ->
+; core_halted : 
+    forall cd mu c1 m1 c2 m2 v1,
+    match_state cd mu c1 m1 c2 m2 ->
+    halted Sem1 c1 = Some v1 ->
+    exists v2, 
+    Mem.inject (as_inj mu) m1 m2 
+    /\ val_inject (restrict (as_inj mu) (vis mu)) v1 v2 
+    /\ halted Sem2 c2 = Some v2 
 
-      exists v2, 
-             Mem.inject (as_inj mu) m1 m2 /\
-             val_inject (restrict (as_inj mu) (vis mu)) v1 v2 /\
-             halted Sem2 c2 = Some v2;
 
-    core_at_external : 
-      forall cd mu c1 m1 c2 m2 e vals1 ef_sig,
-        match_state cd mu c1 m1 c2 m2 ->
-        at_external Sem1 c1 = Some (e,ef_sig,vals1) ->
-        Mem.inject (as_inj mu) m1 m2 /\ 
+; core_at_external : 
+    forall cd mu c1 m1 c2 m2 e vals1 ef_sig,
+    match_state cd mu c1 m1 c2 m2 ->
+    at_external Sem1 c1 = Some (e,ef_sig,vals1) ->
+    Mem.inject (as_inj mu) m1 m2 
+    /\ exists vals2, 
+       Forall2 (val_inject (restrict (as_inj mu) (vis mu))) vals1 vals2 
+       /\ at_external Sem2 c2 = Some (e,ef_sig,vals2)
 
-         exists vals2, 
-            Forall2 (val_inject (restrict (as_inj mu) (vis mu))) vals1 vals2 /\ 
-            at_external Sem2 c2 = Some (e,ef_sig,vals2)
     /\ forall
        (pubSrc' pubTgt' : block -> bool)
        (pubSrcHyp : pubSrc' =
@@ -193,13 +163,13 @@ Module SM_simulation. Section SharedMemory_simulation_inject.
                   locBlocksTgt mu b && REACH m2 (exportedTgt mu vals2) b))
        nu (Hnu: nu = (replace_locals mu pubSrc' pubTgt')),
        match_state cd nu c1 m1 c2 m2 
-       /\ Mem.inject (shared_of nu) m1 m2; 
+       /\ Mem.inject (shared_of nu) m1 m2
 
-    eff_after_external: 
-      forall cd mu st1 st2 m1 e vals1 m2 ef_sig vals2 e' ef_sig'
-        (MemInjMu: Mem.inject (as_inj mu) m1 m2)
-        (MatchMu: match_state cd mu st1 m1 st2 m2)
-        (AtExtSrc: at_external Sem1 st1 = Some (e,ef_sig,vals1))
+; eff_after_external: 
+    forall cd mu st1 st2 m1 e vals1 m2 ef_sig vals2 e' ef_sig'
+      (MemInjMu: Mem.inject (as_inj mu) m1 m2)
+      (MatchMu: match_state cd mu st1 m1 st2 m2)
+      (AtExtSrc: at_external Sem1 st1 = Some (e,ef_sig,vals1))
 
         (* We include the clause AtExtTgt to ensure that vals2 is
          uniquely determined. We have e=e' and ef_sig=ef_sig' by the
@@ -209,21 +179,20 @@ Module SM_simulation. Section SharedMemory_simulation_inject.
          functional in the case where the left value is Vundef. (And
          we need to keep ValInjMu since vals2 occurs in pubTgtHyp) *)
 
-        (AtExtTgt: at_external Sem2 st2 = Some (e',ef_sig',vals2)) 
+      (AtExtTgt: at_external Sem2 st2 = Some (e',ef_sig',vals2)) 
+      (ValInjMu: Forall2 (val_inject (restrict (as_inj mu) (vis mu))) vals1 vals2)  
 
-        (ValInjMu: Forall2 (val_inject (restrict (as_inj mu) (vis mu))) vals1 vals2)  
-
-        pubSrc' 
-        (pubSrcHyp: 
-           pubSrc' 
-           = (fun b => locBlocksSrc mu b && REACH m1 (exportedSrc mu vals1) b))
+      pubSrc' 
+      (pubSrcHyp: 
+         pubSrc' 
+         = (fun b => locBlocksSrc mu b && REACH m1 (exportedSrc mu vals1) b))
         
-        pubTgt' 
-        (pubTgtHyp: 
-           pubTgt' 
-           = fun b => locBlocksTgt mu b && REACH m2 (exportedTgt mu vals2) b)
+      pubTgt' 
+      (pubTgtHyp: 
+         pubTgt' 
+         = fun b => locBlocksTgt mu b && REACH m2 (exportedTgt mu vals2) b)
 
-        nu (NuHyp: nu = replace_locals mu pubSrc' pubTgt'),
+      nu (NuHyp: nu = replace_locals mu pubSrc' pubTgt'),
 
       forall nu' ret1 m1' ret2 m2'
         (HasTy1: Val.has_type ret1 (proj_sig_res (AST.ef_sig e)))
@@ -264,8 +233,7 @@ Module SM_simulation. Section SharedMemory_simulation_inject.
         exists cd', exists st1', exists st2',
           after_external Sem1 (Some ret1) st1 = Some st1' /\
           after_external Sem2 (Some ret2) st2 = Some st2' /\
-          match_state cd' mu' st1' m1' st2' m2'
-}.
+          match_state cd' mu' st1' m1' st2' m2' }.
 
 End SharedMemory_simulation_inject. 
 
